Let $\S$ be a totally ordered set with a binary relation $<$.
For any $x,y \in \S$, we can define the less-than and the equality functions as follows.
\begin{align*}
  \LT_\S(x,y) = 
  \begin{cases}
    1, & \text{if } x < y; \\
    0, & \text{if } x \ge y, \\
  \end{cases}
  \qquad
  \EQ_\S(x,y) = 
  \begin{cases}
    1, & \text{if } x = y; \\
    0, & \text{if } x \neq y. \\
  \end{cases}
\end{align*}
If $\S$ is a complete set of representatives of a finite field $\F_\fieldcard$, then the equality function can be easily realized using the principal character of $\F_\fieldcard$, namely $\EQ_\S(x,y) = 1 - \princhar_\fieldcard(x-y)$.
Since this function is independent of the choice of $\S$, we can write
\begin{align*}
  \EQ_{\F_{\fieldcard}}(x,y) = 1 - \princhar_\fieldcard(x-y).
\end{align*}

\subsection{$2$-variate interpolation of $\LT_\S$.}

  The less-than function can be interpolated using Lemma~\ref{lem:interpolation} and the following truth table
  \begin{align*}
    \begin{array}{c|ccccc}
      < & a_0 & a_1 & a_2 & \cdots & a_{\fieldcard-1} \\
      \hline
      a_0 & 0 & 1 & 1 & \cdots & 1 \\
      a_1 & 0 & 0 & 1 & \cdots & 1 \\
      a_2 & 0 & 0 & 0 & \cdots & 1 \\
      \vdots & \vdots & \vdots & \vdots & \ddots & \vdots \\
      a_{\fieldcard-1} & 0 & 0 & 0 & \cdots & 0 \\
    \end{array}
  \end{align*}
  where $a_i \in \S$ for any $i \in [0,\fieldcard-1]$ and $a_i < a_j$ if $i < j$.
  In particular,
  \begin{align}\label{eq:less_than_function}
    \LT_\S(x,y) &= \sum_{a,b \in \S} \LT_\S(a,b) (1-\princhar_\fieldcard(x - a)) (1-\princhar_\fieldcard(y - b)) \nonumber\\
    &= \sum_{a \in \S} (1-\princhar_\fieldcard(x - a)) \sum_{b \in \S} \LT_\S(a,b)  (1-\princhar_\fieldcard(y - b)) \nonumber\\
    &= \sum_{a \in \S} (1-\princhar_\fieldcard(x - a)) \sum_{b \in \S, a < b} (1-\princhar_\fieldcard(y - b)).
  \end{align}
  In contrast to equality, this function depends on the choice of $\S$.
  Nevertheless, we can fix a certain $\S$ as the default complete set of representatives of $\F_{\fieldcard}$ and denote $\LT_\S(x,y)$ as $\LT_{\F_\fieldcard}(x,y)$.
  For example, $\S$ can be $[0,q-1]$ if $q$ is a prime number.

  Let $p$ be a prime number ans $\S = [0,p-1]$.
  Then $\LT_\S$ has total degree $p$ as proven in Theorem~\ref{lem:less_than_total_degree}.
  To prove this statement we need the following lemmata.

  \begin{lemma}\label{lem:difference_to_p-1}
    \[
      (a - b)^{p-1} = \sum_{i=0}^{p-1} a^i b^{p-1-i} \mod p.
    \]
  \end{lemma}
  \begin{proof}
    Using the binomial theorem we obtain
    \[
      (a - b)^{p-1} = \sum_{i=0}^{p-1} \binom{p-1}{i} a^i (-b)^{p-1-i}.
    \]
    Computing the binomial coefficient modulo $p$
    \begin{align*}
      \binom{p-1}{i} & = \frac{(p-1)!}{i! (p-1-i)!} \\
      & = \frac{(p-1)(p-2)\dots(i+1)}{1 \cdot 2 \dots (p-(1+i))} = (-1)^{p-1-i} \mod p\,,
    \end{align*}
    we prove the lemma.
  \end{proof}

  \begin{lemma}\label{lem:sum_poly}
    Let $P(x)$ be a polynomial of degree $d$ less than $p-1$.
    For any prime number $p > 2$, it holds
    \[
      \sum_{a=0}^{p-1} P(a) = 0 \mod p.
    \]
  \end{lemma}
  \begin{proof}
    It is enough to prove that the sum $\sum_{a=0}^{p-1} a^n = 0 \mod p$ for any $n < p-1$.
    Let $g$ be a primitive element of $\F_p$.
    Since $p > 2$, we have $g \ne 1$.
    Thus, we can rewrite the above sum as follows.
    \begin{align}
      \sum_{i=1}^{p-1} g^{in} = \frac{g^{pn} - g^n}{g^n - 1}.
    \end{align}
    Since $g^{pn} \equiv g^n \mod p$, the sum turns into zero modulo $p$.
  \end{proof}

  \begin{theorem} \label{lem:less_than_total_degree}
    Let $p$ be a prime number bigger than $2$ and $\S = [0,p-1]$, then $\LT_\S$ is a polynomial over $\F_p$ of the following form
    \begin{align*}
      \LT_\S(x,y) = y^{p-1} - \frac{p-1}{2} (xy)^{\frac{p-1}{2}} + \sum_{i,j>0, i+j \le p} a_{ij} x^i y^j 
    \end{align*}
    for some $a_{ij} \in \F_p$.
  \end{theorem}
  \begin{proof}
    Assume that all computations are done modulo $p$.
    Using Lemma~\ref{lem:difference_to_p-1}, we obtain
    \begin{align*}
      \LT_\S(x,y) &=  \sum_{a = 0}^{p-2} \left(1-\sum_{i=0}^{p-1} x^i a^{p-1-i}\right) \sum_{b=a+1}^{p-1} \left(1-\sum_{j=0}^{p-1} y^j b^{p-1-j}\right)\\
    \end{align*}
    Let us expand this expression distributively.
    \begin{align*}
      \sum_{a = 0}^{p-2} \sum_{b=a+1}^{p-1} 1 - \sum_{i=0}^{p-1} x^i a^{p-1-i} - \sum_{i=0}^{p-1} y^i b^{p-1-i} + \sum_{i=0}^{p-1} \sum_{j=0}^{p-1} x^i y^j a^{p-1-i} b^{p-1-j}.
    \end{align*}
    Let us separately compute polynomial coefficients.
    The constant term is equal to
    \begin{align*}
      \sum_{a = 0}^{p-2} \sum_{b=a+1}^{p-1} 1 - a^{p-1} - b^{p-1} + a^{p-1} b^{p-1} = \sum_{a = 0}^{p-2} \sum_{b=a+1}^{p-1} 1 - a^{p-1} - 1 + a^{p-1} = 0 
    \end{align*}
    The coefficients by $x^i$ with $i > 0$ can be computed as follows
    \begin{align*}
      \sum_{a = 0}^{p-2} \sum_{b=a+1}^{p-1} \left(-a^{p-1-i}\right) + a^{p-1-i} = 0.
    \end{align*}
    Next, we compute the coefficients by $y^i$ with $i > 0$.
    \begin{align*}
      -\sum_{a = 0}^{p-2} \sum_{b=a+1}^{p-1} b^{p-1-i} - a^{p-1} b^{p-1-i} &= -\sum_{b=1}^{p-1} b^{p-1-i} - \sum_{a = 1}^{p-2} \sum_{b=a+1}^{p-1} b^{p-1-i} - b^{p-1-i} \\
      &= -\sum_{b=1}^{p-1} b^{p-1-i}.
    \end{align*}
    If $i = p-1$, this sum is equal to $1$.
    According to Lemma~\ref{lem:sum_poly}, it is $0$ if $i \ne 0 \mod (p-1)$.
    
    To compute coefficients by $x^i y^j$ with $i, j > 0$, we will use Faulhaber's formula below
    \begin{align*}
      \sum_{k=1}^n k^e = \frac{1}{e+1} \sum_{i=1}^{e+1} (-1)^{\delta_{ie}} \binom{e+1}{i} B_{e+1-i} \cdot n^i\,,
    \end{align*}
    where $\delta_{ie}$ is the Kronecker delta and $B_{i}$ is the $i$th Bernoulli number.
    This implies that there exist a polynomial $P(x) \in \F_p[X]$ of degree $e+1$ such that
    \begin{align}\label{eq:faulhaber}
      \sum_{k=1}^n k^e = P(n).
    \end{align}
    Note that $P(0) = 0$.
    The coefficient by $x^i y^j$ for some positive $i$ and $j$ is equal to
    \begin{align*}
      \sum_{a = 0}^{p-2} \sum_{b=a+1}^{p-1} a^{p-1-i} b^{p-1-j} = \sum_{b = 1}^{p-1} b^{p-1-j} \sum_{a=0}^{b-1} a^{p-1-i}.
    \end{align*}
    According to~(\ref{eq:faulhaber}), it follows that there exist a polynomial $P(x)$ of degree $p-i$ such that $\sum_{a=0}^{b-1} a^{p-1-i} = P(b)$.
    Since $Q(x) = x^{p-1-j} P(x)$ has degree $2p-1-i-j$, Lemma~\ref{lem:sum_poly} implies that if $i+j > p$, then
    \begin{align*}
      \sum_{b = 1}^{p-1} b^{p-1-j} \sum_{a=0}^{b-1} a^{p-1-i} = \sum_{b=1}^{p-1} Q(b) = 0.
    \end{align*}
    Thus, the total degree of $\LT_\S$ is at most $p$.

    In addition, we consider the case when $i = j$.
    Let us consider the following sum
    \begin{align*}
      \sum_{a=0}^{p-1} a^{p-1-i} \sum_{b=0}^{p-1} b^{p-1-i} = 0.
    \end{align*}
    We can rewrite it as follows
    \begin{align*}
      \sum_{a=0}^{p-1} a^{p-1-i} \sum_{b=0}^{p-1} b^{p-1-i} = 2\sum_{a=0}^{p-2} a^{p-1-i} \sum_{b=a+1}^{p-1} b^{p-1-i} + \sum_{a=0}^{p-1} a^{2(p-1-i)}.
    \end{align*}
    If $i \ne (p-1)/2$, then the last sum is zero.
    Thus, the coefficient by $x^i y^i$ is equal to $\sum_{a=0}^{p-2} a^{p-1-i} \sum_{b=a+1}^{p-1} b^{p-1-i} = 0$.
    If $i = (p-1)/2$, then following the above argument, this coefficient is equal to $-(p-1)/2$.
  \end{proof}

\subsection{$1$-variate interpolation of $\LT_\S$}
  Another way to compare $x$ and $y$ from $\S$ is to compute the difference $x-y$ and find its sign.
  To compute the sign function (or $\LT_\S(z,0)$) using finite field arithmetic, we need to split finite field elements into two classes:  negative ($\F_p^-$) and non-negative ($\F_p^+$).
  In addition, for any $x, y \in \S$ the following property should hold
  \begin{align*}
    x - y \in 
    \begin{cases}
      \F_p^+ \text{ if } \LT_\S(x,y) = 0 \\
      \F_p^- \text{ if } \LT_\S(x,y) = 1
    \end{cases}
  \end{align*}   
  Let $\S = [0, (p-1)/2]$.
  In this case, $\F_p^+ = [0, (p-1)/2]$ and $\F_p^- = [-(p-1)/2, -1]$.

  \todo{finish description of the circuit, prove its polynomial form}
  \begin{align*}
    \IsNegative_\S(z) = \sum_{a=-\frac{p-1}{2}}^{-1} 1 - (z - a)^{p-1}
  \end{align*}

  \begin{align*}
    \sum_{a=-\frac{p-1}{2}}^{-1} 1 - (z - a)^{p-1} &= \sum_{a=-\frac{p-1}{2}}^{-1} 1 - \sum_{i=0}^{p-1} z^i a^{p-1-i} \\
    &= \sum_{i=1}^{p-1} z^i \sum_{a=-\frac{p-1}{2}}^{-1} (-a^{p-1-i})
  \end{align*}
  If $i$ is even, then the $i$th coefficient is
  \begin{align*}
    -\sum_{a=-\frac{p-1}{2}}^{-1} a^{p-1-i} &= -\sum_{a=1}^{\frac{p-1}{2}} a^{p-1-i} = -\frac{\sum_{a=-\frac{p-1}{2}}^{\frac{p-1}{2}} a^{p-1-i}}{2}.
  \end{align*}
  Since $\sum_{a=0}^{p-1} a^{p-1-i} = 0$ if $i \ne p-1$, this coefficient is equal to $0$. 
  If $i = p-1$, then the $i$th coefficient is $-(p-1)/2 = (p+1)/2$.
  If $i$ is odd, then we can rewrite the $i$th coefficient in the following way
  \begin{align*}
    -\sum_{a=-\frac{p-1}{2}}^{-1} a^{p-1-i} &= \sum_{a=1}^{\frac{p-1}{2}} a^{p-1-i}.
  \end{align*}
  As a result, we can write the polynomial of $\IsNegative_\S(z)$ is as follows
  \begin{align*}
    \IsNegative_\S(z) = \frac{p+1}{2} z^{p-1} + \sum_{i=1, \text{odd}}^{p-2} z^i \sum_{a=1}^{\frac{p-1}{2}} a^{p-1-i}.
  \end{align*}

\subsection{Lexicographic order}
  Let $\vx=(x_0,x_1,\ldots,x_{\ell-1})$ and $\vy=(y_0,y_1,\ldots,y_{\ell-1}) \in \F_\fieldcard^\ell$ for the lexicographical order $<$ defined by the choice of $\S$:
  \begin{align*}
    \vx < \vy \Leftrightarrow \exists i\in[0,\ell-1] \text{ such that } x_i < y_i \text{ and } \forall j > i ~~ x_j = y_j\,.
  \end{align*}
  This order induces a function $\LT_{\F_\fieldcard}(\vx, \vy)$ that returns $1$ if $\vx < \vy$ and $0$ otherwise. 
  As done in~\cite{TLWRK20}, we can employ $\EQ_{\F_\fieldcard}$ and $\LT_{\F_\fieldcard}$ to compute $\LT_{\F_\fieldcard}(\vx, \vy)$ as follows
  \begin{align*}
    \LT_{\F_\fieldcard}(\vx, \vy) = \sum_{i=0}^{\ell-2} \LT_{\F_\fieldcard}(x_{i}, y_{i}) \prod_{j=i+1}^{\ell-1} \EQ_{\F_\fieldcard}(x_{j}, y_{j}) + \LT_{\F_\fieldcard}(x_{\ell-1}, y_{\ell-1}).
  \end{align*}
  Notice that the multiplicative depth of this function solely depends on the products of the equality functions.
  In fact, these products compare subvectors $\vx_i = (x_i, x_{i+1},\dots,x_{\ell-1})$ and $\vy_i = (y_i, y_{i+1},\dots,y_{\ell-1})$ for $i \in [1,\ell-1]$.
  Thus, we can rewrite $\LT_{\F_\fieldcard}$ as
  \begin{align}\label{eq:general_lex_order}
    \LT_{\F_\fieldcard}(\vx, \vy) = \sum_{i=0}^{\ell-2} \LT_{\F_\fieldcard}(x_{i}, y_{i}) \EQ_{\F_\fieldcard}(\vx_{i+1}, \vy_{i+1}) + \LT_{\F_\fieldcard}(x_{\ell-1}, y_{\ell-1})
  \end{align}
  with the equality function $\EQ_{\F_\fieldcard}(\vx_{i+1}, \vy_{i+1})$ that returns $1$ if $\vx_{i+1} = \vy_{i+1}$ and $0$ otherwise.
  As shown in~\todo{cite our work}, this function can be realized by a constant-depth circuit in the following way.
  \begin{align}\label{eq:rand_eq_circuit}
    \EQ_{\F_\fieldcard, e}(\vx_{i+1},\vy_{i+1}) = 1 - \princhar_{\fieldcard^e}\left(\sum_{j=i+1}^{\ell-1} r_j (x_j - y_j)\right)
  \end{align}
  where $r_j$ are uniformly random elements from $\F_{\fieldcard^e}$.
  This circuit is false-biased with error probability $\fieldcard^{-e}$.
  We can compute all $\EQ_{\F_\fieldcard, e}(\vx_{i+1},\vy_{i+1})$ using the same number of multiplications as for the single equality using Algorithm~\ref{alg:vector_equalities_circuit}.\todo{What is the complexity?}
  \begin{algorithm}[t]
    \KwIn{
    $\ct_\vx$ -- a ciphertext encrypting $\vx \in \F^\ell_\fieldcard$,
    $\ct_\vy$ -- a ciphertext encrypting $\vy \in \F^\ell_\fieldcard$.
    }
    \KwOut{$\ct$ -- a ciphertext containing the output of $\EQ_{\F_\fieldcard, e}(\vx_{i+1},\vy_{i+1})$ in the $i$th SIMD slot}
    $\ct_1 \leftarrow \Shift(\ct_\vx, 1)$ // removes the value $x_0$ and shifts $\vx$ to the left\\
    $\ct_2 \leftarrow \Shift(\ct_\vy, 1)$ // removes the value $y_0$ and shifts $\vy$ to the left\\
    $\ct \leftarrow \Sub(\ct_1, \ct_2)$ // $(x_i - y_i), i \in [1,\ell-1]$\\
    $r_0,r_1,\dots,r_{\ell-1} \leftarrow \udist(\F_{\fieldcard^e})$ //\todo{define uniform distribution}\\ 
    $\pt_r \leftarrow \pt(r_0,r_1,\dots,r_{\ell-1})$\\
    $\ct \leftarrow \ct \cdot \pt_r$ // $r_i(x_i - y_i), i \in [1,\ell-1]$\\
    $k \leftarrow 1$// $\sum_{j=i}^{\ell-1} r_i(x_i - y_i), i \in [1,\ell-1]$\\
    \While{$k < \ell-1$}{
      $\ct_{tmp} \leftarrow \Shift(\ct, k)$\\
      $\ct \leftarrow \ct + \ct_{tmp}$\\
      $k \leftarrow 2k$\\
    }
    $\ct \leftarrow \Power(\ct, \fieldcard^e-1)$ //$\princhar_{\fieldcard^e}\left(\sum_{j=i}^{\ell-1} r_i(x_i - y_i)\right), i \in [1,\ell-1]$ \\
    $\ct \leftarrow 1 - \ct$\\
    \textbf{Return} $\ct$.
    \caption{Homomorphic circuit computing $\EQ_{\F_\fieldcard, e}(\vx_{i+1},\vy_{i+1})$ in parallel.}\label{alg:vector_equalities_circuit}
  \end{algorithm}
  
  Let us go back to the lexicographic order in equation~(\ref{eq:general_lex_order}).
  Assume that we have a ciphertext $\ct_{\LT}$ containing $\LT_{\F_\fieldcard}(x_i, y_i)$ in the $i$th slot (\todo{elaborate on that}) and the output $\ct_{\EQ}$ of Algorithm~\ref{alg:vector_equalities_circuit}.
  We set the $\ell-1$ slot of $\ct_{\EQ}$ to $1$ and multiply it by $\ct_{\LT}$.
  The resulting ciphertext contains all the products $\LT_{\F_\fieldcard}(x_{i}, y_{i}) \EQ_{\F_\fieldcard}(\vx_{i+1}, \vy_{i+1})$ for any $i \in [0,\ell-2]$ and $\LT_{\F_\fieldcard}(x_{\ell-1}, y_{\ell-1})$, which can be summed in the same way as in the while circuit of Algorithm~\ref{alg:vector_equalities_circuit}.
  As a result, we obtain a ciphertext with the output of $\LT_{\F_\fieldcard}(\vx, \vy)$ in the first SIMD slot.

  \subsubsection{Comparing large integers.}
  Since any integer $z$ can be represented in base $\fieldcard$ as $z = \sum_{i=0}^{\ell-1} z_i q^i$, we can encode $z$ into SIMD slots as a vector $(z_0,z_1,\dots,z_{\ell-1}) \in \F_{\fieldcard}^\ell$.
  As shown above, we can compare such vectors using the lexicographic order function in~(\ref{eq:general_lex_order}) and thus compare integers larger than $\fieldcard$.

  \todo{Incorporate the following into the complexity analysis.} 
  We can obtain ciphertexts encrypting $(x,x,\ldots, x)$ and $(y,y,\ldots, y)$ with $2\log_2(q-1)\texttt{Rot}$ and $2\log_2(q-1)\texttt{Add}$. 

  From there we can obtain encryptions of $(x,x-1,\ldots, x-q-2)$ and $(y-1,y-2,\ldots, y-q-1)$ with $2\texttt{Add}$. We can apply $f$ to these vectors in parallel with a depth of $\log (p-1) + \log d$ for a cost of $2(\log (p-1) + wt(p-1) + d - 2) \texttt{Mult}$. This can be minimized by choosing $p = 2^d + 1$ for some $d$.

  With $2$ more $\texttt{Sub}$ we obtain encryptions of $(1-f(x), 1-f(x-1), \ldots, 1-f(x-q-2))$ and $(1-f(y-1), 1-f(y-2), \ldots, 1-f(y-q-1))$. From there we can get an encryption of the different partial sums in $\log_2(q-1)\texttt{Rot}$, $\log_2(q-1)\texttt{Select}$ and $\log_2(q-1)\texttt{Add}$. The algorithm works as follow:

  \begin{center}
    \begin{tikzpicture}[scale=0.8]
      \newcommand\y{-4};
      
      \draw (0,2) -- (16,2);
      \draw (0,0) -- (16,0);    
      \foreach \x in {0,...,8}{
        \draw (2*\x,0) -- (2*\x,2);
      }
      \foreach \x in {0,...,7}{
        \node at (2*\x+1,1) {$x_\x$};
      }

      \draw (0,2+\y) -- (16,2+\y);
      \draw (0,\y) -- (16,\y);    
      \foreach \x in {0,...,8}{
        \draw (2*\x,0+\y) -- (2*\x,2+\y);
      }

      \node at (1,1+\y) {$x_0 + x_1$};
      \node at (3,1+\y) {$x_1 + x_2$};
      \node at (5,1+\y) {$x_2 + x_3$};
      \node at (7,1+\y) {$x_3 + x_4$};
      \node at (9,1+\y) {$x_4 + x_5$};
      \node at (11,1+\y) {$x_5 + x_6$};
      \node at (13,1+\y) {$x_6 + x_7$};
      \node at (15,1+\y) {$x_7$};

      %%%%%%%%%%%%%%%%%%%%%%%%%%%%%%%%%%%%
      
      \draw (0,2+2*\y) -- (16,2+2*\y);
      \draw (0,0+2*\y) -- (16,0+2*\y);    
      \foreach \x in {0,...,8}{
        \draw (2*\x,0+2*\y) -- (2*\x,2+2*\y);
      }

      \node at (1,1+2*\y) {$\begin{array}{c}
          x_0 + x_1  \\
          + x_2 + x_3
        \end{array}$};
      \node at (3,1+2*\y) {$\begin{array}{c}
          x_1 + x_2  \\
          + x_3 + x_4
        \end{array}$};
      \node at (5,1+2*\y) {$\begin{array}{c}
          x_2 + x_3  \\
          + x_4 + x_5
        \end{array}$};
      \node at (7,1+2*\y) {$\begin{array}{c}
          x_3 + x_4  \\
          + x_5 + x_6
        \end{array}$};
      \node at (9,1+2*\y) {$\begin{array}{c}
          x_4 + x_5  \\
          +x_6 + x_7
        \end{array}$};
      \node at (11,1+2*\y) {$\begin{array}{c}
          x_5 + x_6  \\
          + x_7
        \end{array}$};
      \node at (13,1+2*\y) {$x_6 + x_7$};
      \node at (15,1+2*\y) {$x_7$};

      %%%%%%%%%%%%%%%%%%%%%%%%%%%%%%%%%%%%%%%%%%
      
      \draw (0,2+3*\y) -- (16,2+3*\y);
      \draw (0,0+3*\y) -- (16,0+3*\y);    
      \foreach \x in {0,...,8}{
        \draw (2*\x,0+3*\y) -- (2*\x,2+3*\y);
      }

      \node at (1,1+3*\y) {$\begin{array}{c}
          x_0 + x_1  \\
                              + x_2 + x_3 \\
                              + x_4 + x_5 \\
                              + x_6 + x_7
        \end{array}$};
      \node at (3,1+3*\y) {$\begin{array}{c}
          x_1 + x_2  \\
                              + x_3 + x_4 \\
                              + x_5 + x_6 \\
                              + x_7 \\
        \end{array}$};
      \node at (5,1+3*\y) {$\begin{array}{c}
          x_2 + x_3  \\
                              + x_4 + x_5 \\
                              + x_6 + x_7
        \end{array}$};
      \node at (7,1+3*\y) {$\begin{array}{c}
          x_3 + x_4  \\
                              + x_5 + x_6 \\
                              +x_7
        \end{array}$};
      \node at (9,1+3*\y) {$\begin{array}{c}
          x_4 + x_5  \\
          +x_6 + x_7
        \end{array}$};
      \node at (11,1+3*\y) {$\begin{array}{c}
          x_5 + x_6  \\
          + x_7
        \end{array}$};
      \node at (13,1+3*\y) {$x_6 + x_7$};
      \node at (15,1+3*\y) {$x_7$};

      \foreach \x in {2,...,8}
      \draw[->,thick = 2pt] (2*\x-0.1-1,2) to[bend right] (2*\x-3+0.1,2);

      \foreach \x in {3,...,8}
      \draw[->,thick = 2pt] (2*\x-0.1-1,2+\y) to[bend right] (2*\x-5+0.1,2+\y);

      \foreach \x in {5,...,8}
      \draw[->,thick = 2pt] (2*\x-0.1-1,2+2*\y) to[bend right] (2*\x-9+0.1,2+2*\y);

  \end{tikzpicture}
  \end{center}

  From there we just have to compute the scalar product of the two vectors with $1\texttt{Mult} + \log_2(q-1)\texttt{Rot} + \log_2(q-1)\texttt{Add}$. \newline

  So overall we can compute $<$ over $\mathbb{F}_q$ for $q = p^d$ in:

  \begin{itemize}
  \item $4\log_2 (q-1) \texttt{Rot}$
  \item $(4\log_2 (q-1) + 4) \texttt{Add}$
  \item $(2(\log (p-1) + wt(p-1) + d - 2) + 1) \texttt{Mult}$
  \item $(\log_2 (q-1) + 1) \texttt{Select}$
  \end{itemize}


%%% Local Variables:
%%% mode: latex
%%% TeX-master: "main"
%%% End:
